\documentclass{article}
\usepackage{amsmath, amssymb}

\begin{document}

\textbf{Encuentra el mcd de \( f(x) \) y \( g(x) \) en \( \mathbb{Q}[x] \).}

Dado:

\[
\begin{aligned}
    f(x) &= x^{10} - 3x^9 + 3x^8 - 11x^7 + 11x^6 - 11x^5 + 19x^4 - 13x^3 + 8x^2 - 9x + 3, \\
    g(x) &= x^6 - 3x^5 + 4x^4 - 9x^3 + 5x^2 - 5x + 2.
\end{aligned}
\]

Aplicamos el \textbf{algoritmo de Euclides}, siguiendo la forma:

\[
\begin{aligned}
    f(x) &= q_1(x) g(x) + r_1(x), \\
    g(x) &= q_2(x) r_1(x) + r_2(x), \\
    r_1(x) &= q_3(x) r_2(x) + r_3(x), \\
    &\vdots \\
    r_{n-1}(x) &= q_n(x) r_n(x) + 0.
\end{aligned}
\]

donde el último residuo distinto de cero, \( r_n(x) \), es el \textbf{máximo común divisor}.


\begin{align*}
    f(x) &= (x^4 - 2x) g(x) + (-2x^7 + 6x^6 - 6x^5 + 6x^4 - 13x^3 + 8x^2 - 9x + 3), \\
    g(x) &= (x^2 + 6x - 19) (-2x^7 + 6x^6 - 6x^5 + 6x^4 - 13x^3 + 8x^2 - 9x + 3) + (19x^4 + 57x^3 + 38x^2 - 23x + 2), \\
    r_1(x) &= (x - 3) (19x^4 + 57x^3 + 38x^2 - 23x + 2) + (x^3 + 2x - 1), \\
    r_2(x) &= q_4(x) (x^3 + 2x - 1) + 0.
\end{align*}

\textbf{Conclusión:} El \textbf{máximo común divisor} de \( f(x) \) y \( g(x) \) en \( \mathbb{Q}[x] \) es:

\[
\mathbf{mcd(f(x), g(x)) = x^3 + 2x - 1.}
\]

\end{document}
